AwsCryptographicMaterialProviders/runtimes/java/src/main/smithy-generated/software/amazon/cryptography/materialproviders/model/CreateRequiredEncryptionContextCMMInput.java
@@ -11,16 +11,16 @@ import software.amazon.cryptography.materialproviders.IKeyring;
 import software.amazon.cryptography.materialproviders.Keyring;
 
 /**
- * Inputs for creating an Expected Cryptographic Materials Manager.
+ * Inputs for creating an Required Encryption Context Cryptographic Materials Manager.
  */
-public class CreateExpectedEncryptionContextCMMInput {
+public class CreateRequiredEncryptionContextCMMInput {
   /**
-   * The Cryprographic Materials Manager that the created Expected Cryptographic Materials Manager will delegate to. Either a Keyring or underlying Cryprographic Materials Manager must be specified.
+   * The Cryprographic Materials Manager that the created Required Encryption Context Cryptographic Materials Manager will delegate to. Either a Keyring or underlying Cryprographic Materials Manager must be specified.
    */
   private final ICryptographicMaterialsManager underlyingCMM;
 
   /**
-   * The Keyring that the created Cryprographic Materials Manager will use to wrap data keys. The created Expected Encryption Context CMM will delegate to a Default Cryptographic Materials Manager created with this Keyring. Either a Keyring or an underlying Cryprographic Materials Manager must be specified as input.
+   * The Keyring that the created Cryprographic Materials Manager will use to wrap data keys. The created Required Encryption Context CMM will delegate to a Default Cryptographic Materials Manager created with this Keyring. Either a Keyring or an underlying Cryprographic Materials Manager must be specified as input.
    */
   private final IKeyring keyring;
 
@@ -29,21 +29,21 @@ public class CreateExpectedEncryptionContextCMMInput {
    */
   private final List<String> requiredEncryptionContextKeys;
 
-  protected CreateExpectedEncryptionContextCMMInput(BuilderImpl builder) {
+  protected CreateRequiredEncryptionContextCMMInput(BuilderImpl builder) {
     this.underlyingCMM = builder.underlyingCMM();
     this.keyring = builder.keyring();
     this.requiredEncryptionContextKeys = builder.requiredEncryptionContextKeys();
   }
 
   /**
-   * @return The Cryprographic Materials Manager that the created Expected Cryptographic Materials Manager will delegate to. Either a Keyring or underlying Cryprographic Materials Manager must be specified.
+   * @return The Cryprographic Materials Manager that the created Required Encryption Context Cryptographic Materials Manager will delegate to. Either a Keyring or underlying Cryprographic Materials Manager must be specified.
    */
   public ICryptographicMaterialsManager underlyingCMM() {
     return this.underlyingCMM;
   }
 
   /**
-   * @return The Keyring that the created Cryprographic Materials Manager will use to wrap data keys. The created Expected Encryption Context CMM will delegate to a Default Cryptographic Materials Manager created with this Keyring. Either a Keyring or an underlying Cryprographic Materials Manager must be specified as input.
+   * @return The Keyring that the created Cryprographic Materials Manager will use to wrap data keys. The created Required Encryption Context CMM will delegate to a Default Cryptographic Materials Manager created with this Keyring. Either a Keyring or an underlying Cryprographic Materials Manager must be specified as input.
    */
   public IKeyring keyring() {
     return this.keyring;
@@ -66,22 +66,22 @@ public class CreateExpectedEncryptionContextCMMInput {
 
   public interface Builder {
     /**
-     * @param underlyingCMM The Cryprographic Materials Manager that the created Expected Cryptographic Materials Manager will delegate to. Either a Keyring or underlying Cryprographic Materials Manager must be specified.
+     * @param underlyingCMM The Cryprographic Materials Manager that the created Required Encryption Context Cryptographic Materials Manager will delegate to. Either a Keyring or underlying Cryprographic Materials Manager must be specified.
      */
     Builder underlyingCMM(ICryptographicMaterialsManager underlyingCMM);
 
     /**
-     * @return The Cryprographic Materials Manager that the created Expected Cryptographic Materials Manager will delegate to. Either a Keyring or underlying Cryprographic Materials Manager must be specified.
+     * @return The Cryprographic Materials Manager that the created Required Encryption Context Cryptographic Materials Manager will delegate to. Either a Keyring or underlying Cryprographic Materials Manager must be specified.
      */
     ICryptographicMaterialsManager underlyingCMM();
 
     /**
-     * @param keyring The Keyring that the created Cryprographic Materials Manager will use to wrap data keys. The created Expected Encryption Context CMM will delegate to a Default Cryptographic Materials Manager created with this Keyring. Either a Keyring or an underlying Cryprographic Materials Manager must be specified as input.
+     * @param keyring The Keyring that the created Cryprographic Materials Manager will use to wrap data keys. The created Required Encryption Context CMM will delegate to a Default Cryptographic Materials Manager created with this Keyring. Either a Keyring or an underlying Cryprographic Materials Manager must be specified as input.
      */
     Builder keyring(IKeyring keyring);
 
     /**
-     * @return The Keyring that the created Cryprographic Materials Manager will use to wrap data keys. The created Expected Encryption Context CMM will delegate to a Default Cryptographic Materials Manager created with this Keyring. Either a Keyring or an underlying Cryprographic Materials Manager must be specified as input.
+     * @return The Keyring that the created Cryprographic Materials Manager will use to wrap data keys. The created Required Encryption Context CMM will delegate to a Default Cryptographic Materials Manager created with this Keyring. Either a Keyring or an underlying Cryprographic Materials Manager must be specified as input.
      */
     IKeyring keyring();
 
@@ -95,7 +95,7 @@ public class CreateExpectedEncryptionContextCMMInput {
      */
     List<String> requiredEncryptionContextKeys();
 
-    CreateExpectedEncryptionContextCMMInput build();
+    CreateRequiredEncryptionContextCMMInput build();
   }
 
   static class BuilderImpl implements Builder {
@@ -108,7 +108,7 @@ public class CreateExpectedEncryptionContextCMMInput {
     protected BuilderImpl() {
     }
 
-    protected BuilderImpl(CreateExpectedEncryptionContextCMMInput model) {
+    protected BuilderImpl(CreateRequiredEncryptionContextCMMInput model) {
       this.underlyingCMM = model.underlyingCMM();
       this.keyring = model.keyring();
       this.requiredEncryptionContextKeys = model.requiredEncryptionContextKeys();
@@ -141,11 +141,11 @@ public class CreateExpectedEncryptionContextCMMInput {
       return this.requiredEncryptionContextKeys;
     }
 
-    public CreateExpectedEncryptionContextCMMInput build() {
+    public CreateRequiredEncryptionContextCMMInput build() {
       if (Objects.isNull(this.requiredEncryptionContextKeys()))  {
         throw new IllegalArgumentException("Missing value for required field `requiredEncryptionContextKeys`");
       }
-      return new CreateExpectedEncryptionContextCMMInput(this);
+      return new CreateRequiredEncryptionContextCMMInput(this);
     }
   }
 }
