AwsCryptographicMaterialProviders/dafny/AwsCryptographicMaterialProviders/Model/AwsCryptographyMaterialProvidersTypes.dfy
@@ -56,7 +56,7 @@ include "../../../../StandardLibrary/src/Index.dfy"
  CreateRawRsaKeyring := [];
  CreateAwsKmsRsaKeyring := [];
  CreateDefaultCryptographicMaterialsManager := [];
- CreateExpectedEncryptionContextCMM := [];
+ CreateRequiredEncryptionContextCMM := [];
  CreateCryptographicMaterialsCache := [];
  CreateDefaultClientSupplier := [];
  InitializeEncryptionMaterials := [];
@@ -84,7 +84,7 @@ include "../../../../StandardLibrary/src/Index.dfy"
  ghost var CreateRawRsaKeyring: seq<DafnyCallEvent<CreateRawRsaKeyringInput, Result<IKeyring, Error>>>
  ghost var CreateAwsKmsRsaKeyring: seq<DafnyCallEvent<CreateAwsKmsRsaKeyringInput, Result<IKeyring, Error>>>
  ghost var CreateDefaultCryptographicMaterialsManager: seq<DafnyCallEvent<CreateDefaultCryptographicMaterialsManagerInput, Result<ICryptographicMaterialsManager, Error>>>
- ghost var CreateExpectedEncryptionContextCMM: seq<DafnyCallEvent<CreateExpectedEncryptionContextCMMInput, Result<ICryptographicMaterialsManager, Error>>>
+ ghost var CreateRequiredEncryptionContextCMM: seq<DafnyCallEvent<CreateRequiredEncryptionContextCMMInput, Result<ICryptographicMaterialsManager, Error>>>
  ghost var CreateCryptographicMaterialsCache: seq<DafnyCallEvent<CreateCryptographicMaterialsCacheInput, Result<ICryptographicMaterialsCache, Error>>>
  ghost var CreateDefaultClientSupplier: seq<DafnyCallEvent<CreateDefaultClientSupplierInput, Result<IClientSupplier, Error>>>
  ghost var InitializeEncryptionMaterials: seq<DafnyCallEvent<InitializeEncryptionMaterialsInput, Result<EncryptionMaterials, Error>>>
@@ -469,9 +469,9 @@ include "../../../../StandardLibrary/src/Index.dfy"
  ensures CreateDefaultCryptographicMaterialsManagerEnsuresPublicly(input, output)
  ensures History.CreateDefaultCryptographicMaterialsManager == old(History.CreateDefaultCryptographicMaterialsManager) + [DafnyCallEvent(input, output)]
  
- predicate CreateExpectedEncryptionContextCMMEnsuresPublicly(input: CreateExpectedEncryptionContextCMMInput , output: Result<ICryptographicMaterialsManager, Error>)
+ predicate CreateRequiredEncryptionContextCMMEnsuresPublicly(input: CreateRequiredEncryptionContextCMMInput , output: Result<ICryptographicMaterialsManager, Error>)
  // The public method to be called by library consumers
- method CreateExpectedEncryptionContextCMM ( input: CreateExpectedEncryptionContextCMMInput )
+ method CreateRequiredEncryptionContextCMM ( input: CreateRequiredEncryptionContextCMMInput )
  returns (output: Result<ICryptographicMaterialsManager, Error>)
  requires
  && ValidState() && ( input.underlyingCMM.Some? ==>
@@ -484,7 +484,7 @@ include "../../../../StandardLibrary/src/Index.dfy"
  modifies Modifies - {History} ,
  (if input.underlyingCMM.Some? then input.underlyingCMM.value.Modifies else {}) ,
  (if input.keyring.Some? then input.keyring.value.Modifies else {}) ,
- History`CreateExpectedEncryptionContextCMM
+ History`CreateRequiredEncryptionContextCMM
  // Dafny will skip type parameters when generating a default decreases clause.
  decreases Modifies - {History} ,
  (if input.underlyingCMM.Some? then input.underlyingCMM.value.Modifies else {}) ,
@@ -496,8 +496,8 @@ include "../../../../StandardLibrary/src/Index.dfy"
  && output.value.Modifies !! {History}
  && fresh(output.value)
  && fresh ( output.value.Modifies - Modifies - {History} - (if input.underlyingCMM.Some? then input.underlyingCMM.value.Modifies else {}) - (if input.keyring.Some? then input.keyring.value.Modifies else {}) ) )
- ensures CreateExpectedEncryptionContextCMMEnsuresPublicly(input, output)
- ensures History.CreateExpectedEncryptionContextCMM == old(History.CreateExpectedEncryptionContextCMM) + [DafnyCallEvent(input, output)]
+ ensures CreateRequiredEncryptionContextCMMEnsuresPublicly(input, output)
+ ensures History.CreateRequiredEncryptionContextCMM == old(History.CreateRequiredEncryptionContextCMM) + [DafnyCallEvent(input, output)]
  
  predicate CreateCryptographicMaterialsCacheEnsuresPublicly(input: CreateCryptographicMaterialsCacheInput , output: Result<ICryptographicMaterialsCache, Error>)
  // The public method to be called by library consumers
@@ -821,11 +821,6 @@ include "../../../../StandardLibrary/src/Index.dfy"
  datatype CreateDefaultCryptographicMaterialsManagerInput = | CreateDefaultCryptographicMaterialsManagerInput (
  nameonly keyring: IKeyring
  )
- datatype CreateExpectedEncryptionContextCMMInput = | CreateExpectedEncryptionContextCMMInput (
- nameonly underlyingCMM: Option<ICryptographicMaterialsManager> ,
- nameonly keyring: Option<IKeyring> ,
- nameonly requiredEncryptionContextKeys: EncryptionContextKeys
- )
  datatype CreateMultiKeyringInput = | CreateMultiKeyringInput (
  nameonly generator: Option<IKeyring> ,
  nameonly childKeyrings: KeyringList
@@ -843,15 +838,20 @@ include "../../../../StandardLibrary/src/Index.dfy"
  nameonly publicKey: Option<seq<uint8>> ,
  nameonly privateKey: Option<seq<uint8>>
  )
+ datatype CreateRequiredEncryptionContextCMMInput = | CreateRequiredEncryptionContextCMMInput (
+ nameonly underlyingCMM: Option<ICryptographicMaterialsManager> ,
+ nameonly keyring: Option<IKeyring> ,
+ nameonly requiredEncryptionContextKeys: EncryptionContextKeys
+ )
  class ICryptographicMaterialsCacheCallHistory {
  ghost constructor() {
  PutCacheEntry := [];
- UpdaterUsageMetadata := [];
+ UpdateUsageMetadata := [];
  GetCacheEntry := [];
  DeleteCacheEntry := [];
 }
  ghost var PutCacheEntry: seq<DafnyCallEvent<PutCacheEntryInput, Result<(), Error>>>
- ghost var UpdaterUsageMetadata: seq<DafnyCallEvent<UpdaterUsageMetadataInput, Result<(), Error>>>
+ ghost var UpdateUsageMetadata: seq<DafnyCallEvent<UpdateUsageMetadataInput, Result<(), Error>>>
  ghost var GetCacheEntry: seq<DafnyCallEvent<GetCacheEntryInput, Result<GetCacheEntryOutput, Error>>>
  ghost var DeleteCacheEntry: seq<DafnyCallEvent<DeleteCacheEntryInput, Result<(), Error>>>
 }
@@ -926,26 +926,26 @@ include "../../../../StandardLibrary/src/Index.dfy"
  ensures PutCacheEntryEnsuresPublicly(input, output)
  ensures unchanged(History)
  
- predicate UpdaterUsageMetadataEnsuresPublicly(input: UpdaterUsageMetadataInput , output: Result<(), Error>)
+ predicate UpdateUsageMetadataEnsuresPublicly(input: UpdateUsageMetadataInput , output: Result<(), Error>)
  // The public method to be called by library consumers
- method UpdaterUsageMetadata ( input: UpdaterUsageMetadataInput )
+ method UpdateUsageMetadata ( input: UpdateUsageMetadataInput )
  returns (output: Result<(), Error>)
  requires
  && ValidState()
  modifies Modifies - {History} ,
- History`UpdaterUsageMetadata
+ History`UpdateUsageMetadata
  // Dafny will skip type parameters when generating a default decreases clause.
  decreases Modifies - {History}
  ensures
  && ValidState()
- ensures UpdaterUsageMetadataEnsuresPublicly(input, output)
- ensures History.UpdaterUsageMetadata == old(History.UpdaterUsageMetadata) + [DafnyCallEvent(input, output)]
+ ensures UpdateUsageMetadataEnsuresPublicly(input, output)
+ ensures History.UpdateUsageMetadata == old(History.UpdateUsageMetadata) + [DafnyCallEvent(input, output)]
  {
- output := UpdaterUsageMetadata' (input);
- History.UpdaterUsageMetadata := History.UpdaterUsageMetadata + [DafnyCallEvent(input, output)];
+ output := UpdateUsageMetadata' (input);
+ History.UpdateUsageMetadata := History.UpdateUsageMetadata + [DafnyCallEvent(input, output)];
 }
  // The method to implement in the concrete class. 
- method UpdaterUsageMetadata' ( input: UpdaterUsageMetadataInput )
+ method UpdateUsageMetadata' ( input: UpdateUsageMetadataInput )
  returns (output: Result<(), Error>)
  requires
  && ValidState()
@@ -954,7 +954,7 @@ include "../../../../StandardLibrary/src/Index.dfy"
  decreases Modifies - {History}
  ensures
  && ValidState()
- ensures UpdaterUsageMetadataEnsuresPublicly(input, output)
+ ensures UpdateUsageMetadataEnsuresPublicly(input, output)
  ensures unchanged(History)
  
  predicate GetCacheEntryEnsuresPublicly(input: GetCacheEntryInput , output: Result<GetCacheEntryOutput, Error>)
@@ -1412,7 +1412,7 @@ include "../../../../StandardLibrary/src/Index.dfy"
  | HMAC(HMAC: AwsCryptographyPrimitivesTypes.DigestAlgorithm)
  | None(None: None)
  type SymmetricSigningKeyList = seq<Secret>
- datatype UpdaterUsageMetadataInput = | UpdaterUsageMetadataInput (
+ datatype UpdateUsageMetadataInput = | UpdateUsageMetadataInput (
  nameonly identifier: seq<uint8> ,
  nameonly bytesUsed: PositiveInteger
  )
@@ -1942,10 +1942,10 @@ include "../../../../StandardLibrary/src/Index.dfy"
  History.CreateDefaultCryptographicMaterialsManager := History.CreateDefaultCryptographicMaterialsManager + [DafnyCallEvent(input, output)];
 }
  
- predicate CreateExpectedEncryptionContextCMMEnsuresPublicly(input: CreateExpectedEncryptionContextCMMInput , output: Result<ICryptographicMaterialsManager, Error>)
- {Operations.CreateExpectedEncryptionContextCMMEnsuresPublicly(input, output)}
+ predicate CreateRequiredEncryptionContextCMMEnsuresPublicly(input: CreateRequiredEncryptionContextCMMInput , output: Result<ICryptographicMaterialsManager, Error>)
+ {Operations.CreateRequiredEncryptionContextCMMEnsuresPublicly(input, output)}
  // The public method to be called by library consumers
- method CreateExpectedEncryptionContextCMM ( input: CreateExpectedEncryptionContextCMMInput )
+ method CreateRequiredEncryptionContextCMM ( input: CreateRequiredEncryptionContextCMMInput )
  returns (output: Result<ICryptographicMaterialsManager, Error>)
  requires
  && ValidState() && ( input.underlyingCMM.Some? ==>
@@ -1958,7 +1958,7 @@ include "../../../../StandardLibrary/src/Index.dfy"
  modifies Modifies - {History} ,
  (if input.underlyingCMM.Some? then input.underlyingCMM.value.Modifies else {}) ,
  (if input.keyring.Some? then input.keyring.value.Modifies else {}) ,
- History`CreateExpectedEncryptionContextCMM
+ History`CreateRequiredEncryptionContextCMM
  // Dafny will skip type parameters when generating a default decreases clause.
  decreases Modifies - {History} ,
  (if input.underlyingCMM.Some? then input.underlyingCMM.value.Modifies else {}) ,
@@ -1970,11 +1970,11 @@ include "../../../../StandardLibrary/src/Index.dfy"
  && output.value.Modifies !! {History}
  && fresh(output.value)
  && fresh ( output.value.Modifies - Modifies - {History} - (if input.underlyingCMM.Some? then input.underlyingCMM.value.Modifies else {}) - (if input.keyring.Some? then input.keyring.value.Modifies else {}) ) )
- ensures CreateExpectedEncryptionContextCMMEnsuresPublicly(input, output)
- ensures History.CreateExpectedEncryptionContextCMM == old(History.CreateExpectedEncryptionContextCMM) + [DafnyCallEvent(input, output)]
+ ensures CreateRequiredEncryptionContextCMMEnsuresPublicly(input, output)
+ ensures History.CreateRequiredEncryptionContextCMM == old(History.CreateRequiredEncryptionContextCMM) + [DafnyCallEvent(input, output)]
  {
- output := Operations.CreateExpectedEncryptionContextCMM(config, input);
- History.CreateExpectedEncryptionContextCMM := History.CreateExpectedEncryptionContextCMM + [DafnyCallEvent(input, output)];
+ output := Operations.CreateRequiredEncryptionContextCMM(config, input);
+ History.CreateRequiredEncryptionContextCMM := History.CreateRequiredEncryptionContextCMM + [DafnyCallEvent(input, output)];
 }
  
  predicate CreateCryptographicMaterialsCacheEnsuresPublicly(input: CreateCryptographicMaterialsCacheInput , output: Result<ICryptographicMaterialsCache, Error>)
@@ -2457,11 +2457,11 @@ include "../../../../StandardLibrary/src/Index.dfy"
  ensures CreateDefaultCryptographicMaterialsManagerEnsuresPublicly(input, output)
 
 
- predicate CreateExpectedEncryptionContextCMMEnsuresPublicly(input: CreateExpectedEncryptionContextCMMInput , output: Result<ICryptographicMaterialsManager, Error>)
+ predicate CreateRequiredEncryptionContextCMMEnsuresPublicly(input: CreateRequiredEncryptionContextCMMInput , output: Result<ICryptographicMaterialsManager, Error>)
  // The private method to be refined by the library developer
 
 
- method CreateExpectedEncryptionContextCMM ( config: InternalConfig , input: CreateExpectedEncryptionContextCMMInput )
+ method CreateRequiredEncryptionContextCMM ( config: InternalConfig , input: CreateRequiredEncryptionContextCMMInput )
  returns (output: Result<ICryptographicMaterialsManager, Error>)
  requires
  && ValidInternalConfig?(config) && ( input.underlyingCMM.Some? ==>
@@ -2482,7 +2482,7 @@ include "../../../../StandardLibrary/src/Index.dfy"
  && output.value.ValidState()
  && fresh(output.value)
  && fresh ( output.value.Modifies - ModifiesInternalConfig(config) - (if input.underlyingCMM.Some? then input.underlyingCMM.value.Modifies else {}) - (if input.keyring.Some? then input.keyring.value.Modifies else {}) ) )
- ensures CreateExpectedEncryptionContextCMMEnsuresPublicly(input, output)
+ ensures CreateRequiredEncryptionContextCMMEnsuresPublicly(input, output)
 
 
  predicate CreateCryptographicMaterialsCacheEnsuresPublicly(input: CreateCryptographicMaterialsCacheInput , output: Result<ICryptographicMaterialsCache, Error>)
